wip in the dafny proof

dafny/list.dfy
@@ -2,7 +2,7 @@ include "mod.dfy"
 
 module List {
 
-    import Mod;
+    import Mod
 
     function sorted(list: seq<nat>): bool {
         forall k : nat :: 1 <= k < |list| ==> list[k] > list[k-1]
@@ -17,7 +17,16 @@ module List {
         forall n,m : nat :: 0 <= n < m < |list| ==> list[n] != list[m]
     }
 
-    function method cycle(list:seq<nat>,pos:nat): nat
+    function isCycle(list: seq<nat>, listCycle: seq<nat>): bool
+        requires |list| > 0;
+        requires |listCycle| >= |list|;
+    {
+        assert forall k : nat :: |list| <= k < |listCycle| ==> Mod.mod(k,|list|) == Mod.mod(k - |list|,|list|);
+        assert forall k : nat :: 0 <= k < |list| ==> Mod.mod(k,|list|) == k;
+        forall k : nat :: 0 <= k < |listCycle| ==> listCycle[k] == list[Mod.mod(k,|list|)]
+    }
+
+    function method cyclePos(list:seq<nat>,pos:nat): nat
         requires |list| > 0;
     {
         var result := Mod.mod(pos, |list|);
@@ -26,23 +35,9 @@ module List {
         result
     }
 
-    function method cycleOld(list:seq<nat>, pos: nat): nat
-        requires |list| > 0;
-    decreases pos;
-    {
-        var result := if ( pos < |list| ) then list[pos] else
-            list[pos % |list|];
-        
-        assert pos < |list| ==> list[pos] == result;
-        assert pos >= |list| ==> result == list[ pos % |list| ];
-
-        result
-    }
-
     method cycleUntil(list:seq<nat>, size: nat, gap: nat) returns (result: seq<nat>) 
         requires |list| > 0;
         ensures |result| == size;
-//        ensures forall pos : nat :: 0 <= pos < |result| ==> ;
         ensures forall pos : nat :: 0 <= pos < |result| ==> result[pos] == list[Mod.mod(pos + gap,|list|)]
     {
         if (size == 0 ) {
@@ -51,47 +46,77 @@ module List {
         } else {
             var key := Mod.mod(gap,|list|);
             Mod.remainderShouldBeSmall(gap, |list|, key);
-            Mod.modList(result, list);
             var current := list[key];
             var others := cycleUntil(list, size - 1, gap + 1);
             result := [current] + others;
         }
     }
-//     method cycleUntil(list:seq<nat>, size: nat) returns (result: seq<nat>)
-//         requires |list| > 0;
-//         ensures |result| == size;
-//         ensures forall pos : nat :: pos <  |list| ==> result[pos] == list[pos];
-// //        ensures forall pos : nat :: |list| < pos < |result| ==> result[pos] == list[cycle(list,pos)];
-//     {
-//         var arr := new nat[size];
-//         var k := 0;
-//         var l := |list|;
-//         var v := Mod.mod(k,|list|);
-//         while (k < size)
-//             decreases size - k;
-//             invariant v < |list|;
-//             invariant v == Mod.mod(k,|list|);
-//             invariant 0 < k < size ==> arr[k] == list[v];
-//             // invariant k < size ==> arr[k] == cycle(list,k);
-//             // invariant forall n: nat :: 0 <= n < k ==> ( n <= arr.Length ==> arr[n] == list[n]);
-//             // invariant k < size && k >= |list| ==> arr[k] == list[ Mod.mod(k, |list|) ];
-//         {
-//             v := Mod.mod(k,|list|);
-//             Mod.remainderShouldBeSmall(k,|list|, v);
-//             Mod.loopList(list,k);
 
-//             assert k >= |list| ==> Mod.mod(k,|list|) == Mod.mod(k-|list|, |list|);
-//             assert k <  |list| ==> Mod.mod(k,|list|) == v == k;
-//             arr[k] := list[ v ];
-//             assert k <  |list| ==> arr[k] == list[k];
-//             assert k >= |list| ==> arr[k] == list[ Mod.mod(k,|list|) ];
-//             k := k + 1;
-//             v := Mod.mod(k,|list|);
-//             Mod.remainderShouldBeSmall(k,|list|, v);
-//             assert v <  |list|;
-//         }
-//         result := arr[..];
-//     }
+    method cycle(list: seq<nat>, m: nat) returns (result: seq<nat>)
+        requires m > 0;
+        requires |list| > 0;
+        ensures |result| == |list| * m;
+        ensures forall pos : nat :: 0 <= pos < |result| ==> result[pos] == list[Mod.mod(pos,|list|)];
+        ensures forall pos : nat :: 0 <= pos < |list|   ==> result[pos] == list[pos];
+    {
+        result := cycleUntil(list, |list| * m, 0);
+        assert |result| >= |list|;
+        assert forall pos : nat :: 0 <= pos < |result| ==> result[pos] == list[Mod.mod(pos,|list|)];
+        assert forall pos : nat :: 0 <= pos < |result| ==> Mod.mod(pos, |list|) < |list|;
+        assert forall pos : nat :: 0 <= pos < |list|   ==> Mod.mod(pos, |list|) == pos;
+        assert forall pos : nat :: 0 <= pos < |list|   ==> result[pos] == list[pos];
+    }
+
+
+    // lemma cycleValueRepeatsEveryM(list: seq<nat>, result: seq<nat>, a: nat, m: nat, n: nat)
+    //     requires |list| > 0;
+    //     requires |result| == |list| * m;
+    //     requires m > 0;
+    //     requires n < m;
+    //     requires a < |list|;
+    //     requires isCycle(list,result);
+    //     ensures a + n * |list| < |result|;
+    //     ensures result[a + n * |list| ] == list[a];
+    // {
+    //     Mod.modAtoBshouldBeEqualToModAPlusBtimesMToB(a, |list|, n);
+    //     var l := |list|;
+    //     assert l > 0;
+    //     assert Mod.mod(a + n * l, l) == a;
+    //     assert |result| == l * m;
+    //     assert n < m;
+    //     assert n * l < m * l;
+    //     assert l + n * l <= m * l;
+    //     assert l + n * l > a + n * l;
+    //     assert result[a + n * l] == list[a];
+    //     assert result[a + n * |list|] == list[a];
+    // }
+
+    lemma cycleByConcat(list: seq<nat>, cycleList: seq<nat>, smallCycle: seq<nat>, m: nat, n: nat, a: nat)
+        requires |list| > 0;
+        requires |cycleList| > |list|;
+        requires |smallCycle| > |list|;
+        requires isCycle(list, cycleList);
+        requires isCycle(list, smallCycle);
+        requires a < |list|;
+        requires |cycleList| == |list| * m;
+        requires |smallCycle| == |cycleList| - |list|;
+        requires |smallCycle| == |list| * ( m - 1 );
+        requires m > 0;
+        requires n < m;
+        ensures cycleList == list + cycleList[|list|..];
+        ensures cycleList == list + smallCycle;
+        ensures sum(cycleList) == sum(list) + sum(smallCycle);
+        // ensures m == 1 ==> sum(cycleList) == sum(list);
+        // ensures m == 1 ==> sum(smallCycle) == 0;
+        // ensures m > 1 ==> sum(cycleList) == sum(list) + sum(smallCycle);
+        // ensures m > 1 ==> sum(cycleList) == sum(list) + sum(smallCycle);
+        // ensures sum(cycleList) == m * sum(list);
+    {
+        Mod.modAtoBshouldBeEqualToModAPlusBtimesMToB(a, |list|, n);
+        assert Mod.mod(a + |list| * n, |list|) == a;
+        assert cycleList[0..|list|] == list;
+        distributiveSum(list,smallCycle);
+    }
 
     function first(list: seq<nat>): nat 
         requires |list| > 0;
@@ -112,23 +137,93 @@ module List {
         list[0] + sum(list[1..])
     }
 
-    lemma sumOfListWithVEqualsSumOfListPlusV(list: seq<nat>, v: nat, k: nat)
-        requires 0 < k < |list|;
-    {
-        // var t := [1];
-        // assert t[0] == 1;
-        // assert t[1..] == [];
-        // assert sum([]) == 0;
 
-        assert sum([v] + list) == v + sum(list) == sum(list) + v;
-        var acc := sum(list[..k]);
-        var acc2 := list[k] + sum(list[..k]);
-        assert acc2 == list[k] + acc;
+    ghost method distributiveSum(a: seq<nat>, b: seq<nat> )
+        ensures sum(a + b) == sum(a) + sum(b); 
+    {
+        assert |a| == 0 && |b| == 0 ==> sum(a) + sum(b) == 0 == sum(a + b);
+        assert |a|  > 0 && |b| == 0 ==> a + b == a;    
+        assert |a|  > 0 && |b| == 0 ==> sum(a) + sum(b) == sum(a) + 0 == sum(a) == sum(a + b);
+        assert |a| == 0 && |b|  > 0 ==> a + b == b;
+        assert |a| == 0 && |b|  > 0 ==> sum(a) + sum(b) == sum(b) + 0 == sum(b) == sum( a + b);
+        assert |a|  > 0 && |b|  > 0 ==> sum(a) + sum(b) == a[0] + sum(a[1..]) + b[0] + sum(b[1..]) == a[0] + b[0] + sum(a[1..]) + sum(b[1..]);
+        assert |a|  > 0 && |b|  > 0 ==> a + b == [a[0]] + (a[1..] + b);
+        assert |a|  > 0 && |b|  > 0 ==> sum(a + b) == sum([a[0]]) + sum(a[1..] + b);
+    }
+
+    lemma divSum(list: seq<nat>, n: nat)
+        requires 0 <= n < |list|;
+        ensures sum(list) == sum(list[0..n]) + sum(list[n..]); 
+    {
+        assert list[0..n] + list[n..] == list;
+        var a := list[0..n];
+        var b := list[n..];
+        distributiveSum(a,b);
+    }
+
+    lemma sumListPlusValue(list: seq<nat>, value: nat)
+        ensures sum(list) + value == sum([value] + list);
+        ensures sum(list) + value == sum(list + [value]);
+        ensures value + sum(list) == sum(list) + value;
+    {
+        assert sum(list) + value == sum([value] + list);
+        var a := list;
+        var b := [value];
+        distributiveSum(a, b);
+    }
+
+    lemma sumMultipleList(list: seq<nat>, cycleList: seq<nat>, m: nat)
+        requires m > 0;
+        requires |list| > 0;
+        requires |cycleList| > 0;
+        requires |cycleList| >= |list|;
+        requires isCycle(list, cycleList);
+        requires |cycleList| == |list| * m;
+        ensures sum(cycleList) == sum(list) * m;
+        decreases cycleList, m;
+    {
+        if m == 1 {
+            assert cycleList == list;
+        } else {
+            var smallCycle := cycleList[|list|..];
+            assert cycleList == list + smallCycle;
+            assert isCycle(list, smallCycle);
+            distributiveSum(list,smallCycle);
+            assert sum(cycleList) == sum(list) + sum(smallCycle);
+            sumMultipleList(list,smallCycle, m-1);
+        }
+    }
+
+    lemma cycleListIsListPlusSmallCycleList(list: seq<nat>, cycleList: seq<nat>, smallCycle: seq<nat>, m: nat)
+        requires |list| > 0;
+        requires |cycleList| >= |list|;
+        requires m > 0;
+        requires isCycle(list, cycleList);
+        requires |cycleList| == |list| * m;
+        requires  smallCycle == cycleList[|list|..];
+        ensures cycleList == list + smallCycle;
+        ensures sum(cycleList) == sum(list) + sum(smallCycle);
+        ensures |smallCycle| > 0 ==> isCycle(list, smallCycle);
+        ensures |smallCycle| == |list| * (m - 1);
+    {
+        distributiveSum(list,smallCycle);
+        assert |cycleList| == |list| * m;
+        assert forall v : nat :: 0 <= v < |list| ==> cycleList[v] == list[v];
+        assert |cycleList| >= |list|;
+        assert cycleList == list + smallCycle;
+        assert |smallCycle| > 0 ==> isCycle(list,smallCycle);
+        assert |smallCycle| == |list| * (m - 1);
+    }
+
+    function isIntegral(list: seq<nat>, initial: nat, listIntegral: seq<nat>): bool
+        requires |list| == |listIntegral|;
+    {
+        forall v: nat :: 0 <= v < |list| ==> listIntegral[v] == sum(list[0..v+1]) + initial
     }
 
     method integral(list: seq<nat>, initial: nat ) returns (result: seq<nat>)
         ensures |list| == |result|;
-        ensures forall v: nat :: 0 <= v < |list| ==> result[v] == sum(list[0..v+1]) + initial;
+        ensures isIntegral(list,initial,result);
     {
         var distance := |list|;
         var arr := new nat[distance];
@@ -149,6 +244,116 @@ module List {
         // array to seq
         result := arr[..];
     }
+
+    function isModList(list: seq<nat>, value: nat, modList: seq<nat>): bool
+    requires |list| == |modList|;
+    requires |list| > 0;
+    requires value > 0;
+    {
+        forall v: nat :: 0 <= v < |list| ==> modList[v] == Mod.mod(list[v], value)
+    }
+
+    function isNotMultiple(list: seq<nat>, value: nat): bool
+    requires value > 0;
+    requires |list| > 0;
+    {
+        forall v: nat :: 0 <= v < |list| ==> Mod.mod(list[v], value) != 0
+    }
+
+    lemma modOfIntegral(
+        list: seq<nat>, 
+        initial: nat, 
+        integralList: seq<nat>, 
+        modIntegralList: seq<nat>, 
+        m: nat, 
+        cycleList: seq<nat>, 
+        integralCycle: seq<nat>,
+        modIntegralCycle: seq<nat>
+    )
+
+    // list is non zero, non empty and the sum of the list is multiple of m
+    requires |list| > 0;
+    requires nonZero(list);
+    requires Mod.mod(sum(list),m) == 0;
+
+    // m is bigger than zero
+    requires m > 0;
+
+    // integral list def
+    requires |integralList| == |list|;
+    requires isIntegral(list, initial, integralList);
+    
+    // mod of integral list def
+    requires |modIntegralList| == |integralList|;
+    requires isModList(integralList, m, modIntegralList);
+
+    // cylce list def
+    requires |cycleList| == |list| * m;
+    requires isCycle(list, cycleList)
+
+    // integral cycle def
+    requires |integralCycle| == |cycleList|;
+    requires isIntegral(cycleList, initial, integralCycle);
+    
+    // mod of integral cycle def
+    requires |modIntegralCycle| == |integralCycle|;
+    requires isModList(integralCycle, m, modIntegralCycle);
+
+    // mod of integral should be cycle
+    ensures isCycle(modIntegralList, modIntegralCycle);
+    {
+        if ( m == 1 ) {
+            assert cycleList == list;
+            assert integralCycle == integralList;
+            assert modIntegralCycle == modIntegralList;
+        } else {
+            assert cycleList[..|list|] == list;
+        }
+    }
+
+    // lemma bigProoff(
+    //     initial: nat,  // 5
+    //     prev: seq<nat>, // [ 2 3 ]
+    //     list: seq<nat>, // [ 2 4 ]
+    //     integralList: seq<nat>, // [ 7 11 ]
+    //     modList: seq<nat>, // [2, 1]
+    //     modIntegralList: seq<nat>, // [1, 2]
+    //     m: nat, // 3
+    //     cycleList: seq<nat>, // [ 2 4 2 4 2 4 ]
+    //     integralCycle: seq<nat>, // [ 7 11 13 17 19 23 ]
+    //     modIntegralCycle: seq<nat> // [ 1 2 1 2 1 2 ]
+    // )
+    //     requires m > 0;
+    //     requires |list| > 0;
+    //     requires nonZero(list);
+    //     requires |cycleList| == |list| * m;
+    //     requires |list| == |integralList|;
+
+    //     requires |modList| == |list|;
+    //     requires isModList(list, m, modList);
+    //     requires nonZero(modList);
+
+    //     requires isIntegral(list, initial, integralList);
+    //     requires isCycle(list, cycleList);
+    //     requires |integralCycle| == |cycleList|;
+    //     requires isIntegral(cycleList, initial, integralCycle);
+
+    //     // // if the list integral is not multiple of m
+    //     requires isNotMultiple(integralList, m);
+    //     requires |modIntegralList| == |integralList|;
+    //     requires isModList(integralList, m, modIntegralList);
+    //     requires nonZero(modIntegralList);
+
+    //     requires |modIntegralCycle| == |integralCycle|;
+    //     requires isModList(integralCycle, m, modIntegralCycle);
+
+    //     requires Mod.mod(sum(list), m) == 0; // [2 4] ==> 2 + 4 == 6 ==> 6 % 3 == 0;
+        
+    //     // the next integral should also be not multiple of m
+    //     ensures isNotMultiple(integralCycle, m);
+    //     ensures nonZero(modIntegralCycle);
+    // {
+    // }
 
     method testIntegral(v:nat, list: seq<nat>, initial: nat)
     {
